theories/TensorCore/Tensor.v
@@ -6,7 +6,70 @@ Set Warnings "-stdlib-vector".
 From stdpp Require vector.
 Import vector.
 
+(* FIXME: Move *)
+Definition vsplitl {A n m} (v : vec A (n + m)) : vec A n :=
+  (Vector.splitat n v).1.
+Definition vsplitr {A n m} (v : vec A (n + m)) : vec A m :=
+  (Vector.splitat n v).2.
+Definition app_vsplit {A n m} (v : vec A (n + m)) :
+  vsplitl v +++ vsplitr v = v.
+Proof.
+  apply symmetry, Vector.append_splitat, surjective_pairing.
+Qed.
+Lemma vsplit_eq {A n m} (v w : vec A (n + m)) : 
+  v = w <-> vsplitl v = vsplitl w /\ vsplitr v = vsplitr w.
+Proof.
+  split; [now intros ->|].
+  intros [Hl Hr].
+  rewrite <- (app_vsplit v), <- (app_vsplit w).
+  congruence.
+Qed.
+Lemma vsplitl_app {A n m} (v : vec A n) (w : vec A m) : 
+  vsplitl (v +++ w) = v.
+Proof.
+  unfold vsplitl.
+  now rewrite Vector.splitat_append.
+Qed.
+Lemma vsplitr_app {A n m} (v : vec A n) (w : vec A m) : 
+  vsplitr (v +++ w) = w.
+Proof.
+  unfold vsplitr.
+  now rewrite Vector.splitat_append.
+Qed.
+
 Require Export SummableWF.
+
+Lemma SummedElement_vec_iff `{Summable A} {n} (v : vec A n) :
+  SummedElement v <-> (forall a, a ∈@{list _} v -> SummedElement a).
+Proof.
+  split; [|apply SummedElement_vec].
+  setoid_rewrite SummedElement_iff.
+  setoid_rewrite elem_of_list_In.
+  intros Hv%vec_elements_in%Vector.to_list_Forall.
+  apply List.Forall_forall.
+  revert Hv.
+  now rewrite vec_to_list_to_list.
+Qed.
+
+Lemma SummedElement_vec_iff_Forall `{Summable A} {n} (v : vec A n) :
+  SummedElement v <-> Forall SummedElement v.
+Proof.
+  now rewrite SummedElement_vec_iff, <- Forall_forall.
+Qed.
+#[export] Instance SummedElement_vsplitl `{Summable A} {n m} (v : vec A (n + m)) :
+  SummedElement v -> SummedElement (vsplitl v).
+Proof.
+  rewrite 2 SummedElement_vec_iff_Forall.
+  rewrite <- (app_vsplit v), vec_to_list_app, Forall_app at 1.
+  easy.
+Qed.
+#[export] Instance SummedElement_vsplitr `{Summable A} {n m} (v : vec A (n + m)) :
+  SummedElement v -> SummedElement (vsplitr v).
+Proof.
+  rewrite 2 SummedElement_vec_iff_Forall.
+  rewrite <- (app_vsplit v), vec_to_list_app, Forall_app at 1.
+  easy.
+Qed.
 
 Definition Tensor {R} (n m : nat) (A : Type) :=
   Vector.t A n -> Vector.t A m -> R.
@@ -64,24 +127,53 @@ Proof.
 Qed.
 
 #[global] Instance StronglyPermutativeTensorLike_PermutativeTensorLike
-  `{SemiRing R rO rI radd rmul req} `(TensT : TensorLike R A T)
+  `{SR : SemiRing R rO rI radd rmul req} `(TensT : TensorLike R A T)
   (SP : StronglyPermutativeTensorLike TensT) : PermutativeTensorLike TensT.
 Proof.
   constructor; intros; apply strongly_permutative_tensor_permutative_tensor,
     interpretTensorStronglyPermutative.
 Qed.
 
-Definition tensoreq `{SemiRing R rO rI radd rmul req} 
-  `{Summable A} {n m} : relation (@Tensor R n m A) :=
-  fun t t' => forall v w, SummedElement v -> SummedElement w -> 
+Definition tensoreq `{SR : SemiRing R rO rI radd rmul req}
+  `{SA : Summable A} {n m} : relation (@Tensor R n m A) :=
+  fun t t' => forall v w, SummedElement v -> SummedElement w ->
     req (t v w) (t' v w).
-
-(* TODO: refl, sym, trans lemmas, and Add Parametric Relation 
-  Also, do we want to factor as summable_relation (same type 
-  as pointwise relation) for better integration? *)
 
 #[global] Instance Tensor_equiv `{SemiRing R rO rI radd rmul req}
   `{Summable A} {n m} : Equiv (@Tensor R n m A) := tensoreq.
+
+Section tensoreq.
+
+Context `{SR : SemiRing R rO rI radd rmul req} `{SA : Summable A}.
+
+Lemma tensoreq_refl {n m} (t : @Tensor R n m A) : t ≡ t.
+Proof. hnf; intros; apply SR. Qed.
+Lemma tensoreq_symm {n m} (t t' : @Tensor R n m A) : t ≡ t' -> t' ≡ t.
+Proof. 
+  intros Ht. 
+  hnf; intros.
+  now apply SR.(Req_equiv).(Equivalence_Symmetric), Ht. 
+Qed.
+Lemma tensoreq_trans {n m} (t t' t'' : @Tensor R n m A) : t ≡ t' -> t' ≡ t'' -> t ≡ t''.
+Proof. 
+  intros Ht Ht'. 
+  hnf; intros.
+  now eapply SR.(Req_equiv).(Equivalence_Transitive); [apply Ht|apply Ht'].
+Qed.
+
+End tensoreq.
+
+Add Parametric Relation `{SR : SemiRing R rO rI radd rmul req}
+  `{SA : Summable A} {n m} : (@Tensor R n m A) tensoreq 
+  reflexivity proved by tensoreq_refl
+  symmetry proved by tensoreq_symm
+  transitivity proved by tensoreq_trans
+  as tensoreq_setoid.
+
+(* TODO: refl, sym, trans lemmas, and Add Parametric Relation
+  Also, do we want to factor as summable_relation (same type
+  as pointwise relation) for better integration? *)
+
 
 Section TensorOps.
 
@@ -89,16 +181,101 @@ Context {R : Type}.
 
 Let Tensor := (@Tensor R).
 
-Definition delta_tensor `{Summable A, EqDecision A, SemiRing R rO rI radd rmul req}
+Definition delta_tensor `{SA : Summable A, EqA : EqDecision A,
+  SR : SemiRing R rO rI radd rmul req}
   {n : nat} : Tensor n n A :=
   fun v w => if decide (v = w) then rI else rO.
 
 
-Definition compose_tensor `{Summable A, SemiRing R rO rI radd rmul req}
+Definition compose_tensor `{SA : Summable A,
+  SR : SemiRing R rO rI radd rmul req}
   {n m o} (t : Tensor n m A) (t' : Tensor m o A) :
   Tensor n o A :=
   fun v w =>
   ∑ u : vec A m, rmul (t v u) (t' u w).
+
+Definition stack_tensor `{SA : Summable A,
+  SR : SemiRing R rO rI radd rmul req}
+  {n m n' m'} (t : Tensor n m A) (t' : Tensor n' m' A) :
+  Tensor (n + n') (m + m') A :=
+  fun v w =>
+  rmul (t (vsplitl v) (vsplitl w)) (t' (vsplitr v) (vsplitr w)).
+
+
+Definition swapped_stack_tensor `{SA : Summable A,
+  SR : SemiRing R rO rI radd rmul req}
+  {n m n' m'} (t : Tensor n m A) (t' : Tensor n' m' A) :
+  Tensor (n' + n) (m + m') A :=
+  fun v w =>
+  rmul (t (vsplitr v) (vsplitl w)) (t' (vsplitl v) (vsplitr w)).
+
+
+Definition join_stack_1_tr_bl `{SA : Summable A,
+  SR : SemiRing R rO rI radd rmul req} {n m o} 
+  (t : Tensor (n + (S m)) ((S m) + o) A) : Tensor (n + m) (m + o) A :=
+  fun v w => 
+  ∑ a : A, t (vsplitl v +++ a ::: vsplitr v) (a ::: w).
+
+Fixpoint join_stack_tr_bl `{SA : Summable A,
+  SR : SemiRing R rO rI radd rmul req} {n m o} : 
+  forall (t : Tensor (n + m) (m + o) A), Tensor n o A :=
+  match m with
+  | 0 => fun t v w => t (v +++ [#]) w
+  | S m => fun t => 
+    join_stack_tr_bl (join_stack_1_tr_bl t)
+  end.
+
+
+Definition join_stack_1_tl_bl `{SA : Summable A,
+  SR : SemiRing R rO rI radd rmul req} {n m} 
+  (t : Tensor (S n) (S m) A) : Tensor n m A :=
+  fun v w => 
+  ∑ a : A, t (a ::: v) (a ::: w).
+
+Fixpoint join_stack_tl_bl `{SA : Summable A,
+  SR : SemiRing R rO rI radd rmul req} {n m o} : 
+  forall (t : Tensor (n + m) (n + o) A), Tensor m o A :=
+  match n with
+  | 0 => fun t => t
+  | S m => fun t => 
+    join_stack_tl_bl (join_stack_1_tl_bl t)
+  end.
+
+#[global] Arguments delta_tensor {_ _ _} {_ _ _ _ _ _} {_} _ _ / : assert.
+#[global] Arguments compose_tensor {_ _} {_ _ _ _ _ _} {_ _ _} (_ _) _ _ / : assert.
+#[global] Arguments stack_tensor {_ _} {_ _ _ _ _ _} {_ _ _ _} (_ _) _ _ / : assert.
+#[global] Arguments swapped_stack_tensor {_ _} {_ _ _ _ _ _} {_ _ _ _} (_ _) _ _ / : assert.
+#[global] Arguments join_stack_1_tr_bl {_ _} {_ _ _ _ _ _} {_ _ _} (_) _ _ / : assert.
+#[global] Arguments join_stack_tr_bl {_ _} {_ _ _ _ _ _} {_ !_ _} (_) / _ _ : assert.
+#[global] Arguments join_stack_1_tl_bl {_ _} {_ _ _ _ _ _} {_ _} (_) _ _ / : assert.
+#[global] Arguments join_stack_tl_bl {_ _} {_ _ _ _ _ _} {!_ _ _} (_) / _ _ : assert.
+
+
+
+Add Parametric Morphism `{SA : Summable A,
+  SR : SemiRing R rO rI radd rmul req} {n m o} :
+    (compose_tensor (SA:=SA) (SR:=SR) (n:=n) (m:=m) (o:=o)) with signature
+    equiv ==> equiv ==> equiv as compose_tensor_mor.
+Proof.
+  intros l l' Hl r r' Hr v w Hv Hw.
+  cbn.
+  apply sum_of_ext'; intros u Hu%SummedElement_iff.
+  apply SR.
+  - now apply Hl.
+  - now apply Hr.
+Qed.
+
+Add Parametric Morphism `{SA : Summable A,
+  SR : SemiRing R rO rI radd rmul req} {n m n' m'} :
+    (stack_tensor (SA:=SA) (SR:=SR) (n:=n) (m:=m) (n':=n') (m':=m')) with signature
+    equiv ==> equiv ==> equiv as stack_tensor_mor.
+Proof.
+  intros l l' Hl r r' Hr v w Hv Hw.
+  cbn.
+  apply SR.
+  - now apply Hl; try apply _.
+  - now apply Hr; try apply _.
+Qed.
 
 
 Section TensorOpFacts.
@@ -165,8 +342,8 @@ Lemma sum_of_delta_r `{!WFSummable A} {n} {w : vec A n}
   `{Hw : !SummedElement w} (f : vec A n -> R) :
   ∑ v : vec A n, delta_tensor w v * f v == f w.
 Proof.
-  setoid_rewrite delta_tensor_comm.
-  apply sum_of_delta_l.
+  rewrite <- sum_of_delta_l.
+  apply sum_of_ext; now intros; rewrite delta_tensor_comm.
 Qed.
 
 
@@ -198,6 +375,92 @@ Proof.
   intros v w Hv Hw.
   unfold compose_tensor.
   now rewrite sum_of_delta_r.
+Qed.
+
+Lemma compose_delta_r `{!WFSummable A} {n m} (t : Tensor n m A) :
+  compose_tensor t delta_tensor ≡ t.
+Proof.
+  intros v w Hv Hw.
+  unfold compose_tensor.
+  setoid_rewrite rmul_comm.
+  now rewrite sum_of_delta_l.
+Qed.
+
+Lemma stack_delta_tensors {n m} : 
+  stack_tensor (delta_tensor (n:=n)) (delta_tensor (n:=m)) ≡
+  delta_tensor.
+Proof.
+  intros v w Hv Hw.
+  unfold stack_tensor.
+  unfold delta_tensor.
+  rewrite (decide_ext _ _ _ _ (vsplit_eq v w)).
+  case_decide; case_decide; case_decide; tauto + ring.
+Qed.
+
+Lemma compose_succ_mid {n m o} (t : Tensor n (S m) A) (t' : Tensor (S m) o A) : 
+  compose_tensor t t' ≡ 
+  fun v w => ∑ a : A, compose_tensor (fun v w => t v (a:::w))
+    (fun v w => t' (a:::v) w) v w.
+Proof.
+  intros v w Hv Hw.
+  cbn.
+  now rewrite sum_of_vec_succ.
+Qed.
+
+Lemma join_stack_tr_bl_alt {n m o} (t : Tensor (n + m) (m + o) A) :
+  join_stack_tr_bl t ≡ fun v w => ∑ u : vec A m, t (v+++u) (u+++w).
+Proof.
+  induction m.
+  - intros v w Hv Hw.
+    cbn. 
+    now rewrite sum_of_vec_0.
+  - cbn. 
+    rewrite IHm. 
+    intros v w Hv Hw.
+    rewrite sum_of_vec_succ, sum_of_comm.
+    apply sum_of_ext; intros u.
+    cbn.
+    apply sum_of_ext; intros a.
+    now rewrite vsplitl_app, vsplitr_app.
+Qed.
+
+Lemma compose_to_stack {n m o} (t : Tensor n m A) (t' : Tensor m o A) : 
+  compose_tensor t t' ≡
+  join_stack_tr_bl (stack_tensor t t').
+Proof.
+  rewrite join_stack_tr_bl_alt.
+  intros v w Hv Hw.
+  cbn.
+  apply sum_of_ext; intros u.
+  now rewrite !vsplitl_app, !vsplitr_app.
+Qed.
+
+
+Lemma join_stack_tl_bl_alt {n m o} (t : Tensor (n + m) (n + o) A) :
+  join_stack_tl_bl t ≡ fun v w => ∑ u : vec A n, t (u+++v) (u+++w).
+Proof.
+  induction n.
+  - intros v w Hv Hw.
+    cbn. 
+    now rewrite sum_of_vec_0.
+  - cbn. 
+    rewrite IHn. 
+    intros v w Hv Hw.
+    cbn.
+    rewrite sum_of_vec_succ, sum_of_comm.
+    reflexivity.
+Qed.
+
+
+Lemma compose_to_swapped_stack {n m o} (t : Tensor n m A) (t' : Tensor m o A) : 
+  compose_tensor t t' ≡
+  join_stack_tl_bl (swapped_stack_tensor t t').
+Proof.
+  rewrite join_stack_tl_bl_alt.
+  intros v w Hv Hw.
+  cbn.
+  apply sum_of_ext; intros u.
+  now rewrite !vsplitl_app, !vsplitr_app.
 Qed.
 
 (* TODO: More *)
