theories/GraphCore/TensorGraphExpr.v
@@ -309,90 +309,6 @@ Proof.
     apply union_subseteq_r.
 Qed.
 
-Lemma relabel_bounds_node_input_edges lint k fint :
-  prod_map fint id <$>
-    (node_input_edges k lint) =
-  node_input_edges k (prod_map fint id <$> lint).
-Proof.
-  unfold node_input_edges.
-  rewrite list_filter_fmap.
-  reflexivity.
-Qed.
-
-Lemma relabel_bounds_node_output_edges lext k fint :
-  prod_map fint id <$>
-    (node_output_edges k lext) =
-  node_output_edges k (prod_map fint id <$> lext).
-Proof.
-  unfold node_output_edges.
-  rewrite list_filter_fmap.
-  reflexivity.
-Qed.
-(*
-Lemma relabel_bounds_input_edges lint lext k fint :
-  relabel_bounds (Pos.of_succ_nat ∘ fint ∘ pos_to_nat_pred) <$>
-    (input_edges lint lext k) =
-  input_edges (prod_map fint id <$> lint) lext k.
-Proof.
-  unfold input_edges.
-  rewrite <- relabel_bounds_node_input_edges.
-  rewrite <- list_fmap_compose, fmap_app, <- !list_fmap_compose.
-  f_equal.
-  now apply list_fmap_ext; intros _ ? _; cbn; rewrite pos_to_nat_pred_of_nat.
-Qed.
-
-Lemma relabel_bounds_output_edges lint lext k fint :
-  relabel_bounds (Pos.of_succ_nat ∘ fint ∘ pos_to_nat_pred) <$>
-    (output_edges lint lext k) =
-  output_edges (prod_map fint id <$> lint) lext k.
-Proof.
-  unfold output_edges.
-  rewrite <- relabel_bounds_node_output_edges.
-  rewrite <- list_fmap_compose, fmap_app, <- !list_fmap_compose.
-  f_equal.
-  now apply list_fmap_ext; intros _ ? _; cbn; rewrite pos_to_nat_pred_of_nat.
-Qed. *)
-
-(*
-Lemma relabel_bounds_mk_node lint lext k fint :
-  relabel_abs (relabel_bounds (Pos.of_succ_nat ∘ fint ∘ pos_to_nat_pred))
-    (mk_node lint lext k) =
-  mk_node (prod_map fint id <$> lint) lext k.
-Proof.
-  unfold mk_node; cbn.
-  now rewrite relabel_bounds_input_edges, relabel_bounds_output_edges.
-Qed. *)
-
-
-(* Lemma relabel_bounds_input_edges' lint lext k fr :
-  relabel_bounds fr <$>
-    (input_edges lint lext k) =
-  input_edges (prod_map (pos_to_nat_pred ∘ fr ∘ Pos.of_succ_nat) id <$> lint) lext k.
-Proof.
-  rewrite <- relabel_bounds_input_edges.
-  apply list_fmap_ext; intros _ ? _; apply relabel_bounds_ext; intros ?;
-  unfold compose; cbn; now rewrite !pos_to_nat_pred_to_pos.
-Qed.
-
-Lemma relabel_bounds_output_edges' lint lext k fr :
-  relabel_bounds fr <$>
-    (output_edges lint lext k) =
-  output_edges (prod_map (pos_to_nat_pred ∘ fr ∘ Pos.of_succ_nat) id <$> lint) lext k.
-Proof.
-  rewrite <- relabel_bounds_output_edges.
-  apply list_fmap_ext; intros _ ? _; apply relabel_bounds_ext; intros ?;
-  unfold compose; cbn; now rewrite !pos_to_nat_pred_to_pos.
-Qed.
-
-Lemma relabel_bounds_mk_node' lint lext k fr :
-  relabel_abs (relabel_bounds fr)
-    (mk_node lint lext k) =
-  mk_node (prod_map (pos_to_nat_pred ∘ fr ∘ Pos.of_succ_nat) id <$> lint) lext k.
-Proof.
-  unfold mk_node; cbn.
-  now rewrite relabel_bounds_input_edges', relabel_bounds_output_edges'.
-Qed. *)
-
 
 Lemma fmap_elements `{FinSet A SA, FinSet B SB} (f : A -> B) `{!Inj eq eq f} (X : SA) :
   f <$> elements X ≡ₚ
@@ -524,8 +440,6 @@ Proof.
   apply Hfr; specialize (HWF.2); [set_solver +Hx|set_solver +Hy].
 Qed. *)
 
-(* FIXME: Move *)
-
 Lemma NoDup_fmap_ind `(f : A -> B) (P : list A -> Prop)
   (Pnil : P []) (Pcons : forall a l, f a ∉ f <$> l -> NoDup (f <$> l) ->
     P l -> P (a :: l)) : forall l, NoDup (f <$> l) -> P l.
@@ -534,39 +448,6 @@ Proof.
   induction l; [easy|].
   cbn; rewrite NoDup_cons.
   intros []; eauto.
-Qed.
-
-Lemma input_edges_ext_label_irrel lint lext lext' k :
-  lext.*2 = lext'.*2 ->
-  input_edges lint lext k = input_edges lint lext' k.
-Proof.
-  intros Hlext.
-  unfold input_edges; f_equal.
-  unfold node_input_edges.
-  rewrite 2 (list_fmap_compose snd), <- 2 list_filter_fmap.
-  now rewrite Hlext.
-Qed.
-
-Lemma output_edges_ext_label_irrel lint lext lext' k :
-  lext.*2 = lext'.*2 ->
-  output_edges lint lext k = output_edges lint lext' k.
-Proof.
-  intros Hlext.
-  unfold output_edges; f_equal.
-  unfold node_output_edges.
-  rewrite 2 (list_fmap_compose snd (_ ∘ snd)), <- 2 list_filter_fmap.
-  now rewrite Hlext.
-Qed.
-
-Lemma mk_node_ext_label_irrel lint lext lext' k :
-  lext.*2 = lext'.*2 ->
-  mk_node lint lext k = mk_node lint lext' k.
-Proof.
-  intros Hext.
-  unfold mk_node.
-  f_equal; [f_equal|];
-  [now apply input_edges_ext_label_irrel|
-   now apply output_edges_ext_label_irrel].
 Qed.
 
 Lemma zip_with_irrel_l {A B C} (f : B -> C) (l l' : list A) (k : list B) :
@@ -585,129 +466,6 @@ Proof.
   intros Hall%Forall2_same_length.
   revert l;
   induction Hall; intros []; cbn; congruence.
-Qed.
-
-Lemma graph_namedtensorlist_semantics_ext_lab_irrel tg int_lab ext_lab ext_lab' :
-  length ext_lab = length ext_lab' ->
-  graph_namedtensorlist_semantics tg int_lab ext_lab =
-  graph_namedtensorlist_semantics tg int_lab ext_lab'.
-Proof.
-  intros Hlen.
-  unfold graph_namedtensorlist_semantics.
-  f_equal.
-  apply list_fmap_ext; intros _ x _.
-  apply mk_node_ext_label_irrel.
-  rewrite 2 fmap_zip_with; cbn.
-  now apply zip_with_irrel_l.
-Qed.
-
-
-
-Lemma graph_namedtensorlist_semantics_perm_eq tg int_lab int_lab'
-  ext_lab ext_lab' :
-  NoDup int_lab -> length int_lab = num_internals tg ->
-  int_lab ≡ₚ int_lab' ->
-  length ext_lab = length ext_lab' ->
-  graph_namedtensorlist_semantics tg int_lab ext_lab =ntl=
-  graph_namedtensorlist_semantics tg int_lab' ext_lab'.
-Proof.
-  intros Hdup Hlen (f & Hf & <- & Hlook)%perm_exists_posperm Hext.
-  etransitivity; [apply graph_namedtensorlist_semantics_ppermute; eauto|].
-  apply eq_reflexivity.
-  now apply graph_namedtensorlist_semantics_ext_lab_irrel.
-Qed.
-
-
-Lemma graph_namedtensorlist_semantics_seq_correct' tg :
-  graph_tensorlist_semantics tg =
-  ntl2tl (graph_namedtensorlist_semantics tg (seq 0 (num_internals tg))
-	  (seq 0 (num_externals tg))).
-Proof.
-  rewrite graph_namedtensorlist_semantics_seq_correct.
-  now rewrite tl2ntl2tl.
-Qed.
-
-Lemma internal_edges_perm ns es es' :
-  es ≡ₚ es' ->
-  @internal_edges T (mk_cohg ns es) ≡ₚ internal_edges (mk_cohg ns es').
-Proof.
-  intros Hes.
-  unfold internal_edges; cbn.
-  now f_equiv.
-Qed.
-
-Lemma external_edges_perm ns es es' :
-  es ≡ₚ es' ->
-  @external_edges T (mk_cohg ns es) ≡ₚ external_edges (mk_cohg ns es').
-Proof.
-  intros Hes.
-  unfold external_edges; cbn.
-  now f_equiv.
-Qed.
-
-
-Lemma graph_tensorlist_semantics_perm_eq_pairs_elab ns es es' :
-  es ≡ₚ es' ->
-  exists idxs idxs',
-  idxs ≡ₚ seq 0 (num_internals (mk_cohg ns es)) /\
-  idxs' ≡ₚ seq 0 (num_externals (mk_cohg ns es)) /\
-  tl2ntl (graph_tensorlist_semantics (mk_cohg ns es)) ≡ntl'≡ₚ
-  graph_namedtensorlist_semantics_aux
-    (zip idxs (internal_edges (mk_cohg ns es')))
-    (zip idxs' (external_edges (mk_cohg ns es')))
-    (map_to_list ns).*1 /\
-  graph_namedtensorlist_semantics_aux
-    (zip idxs (internal_edges (mk_cohg ns es')))
-    (zip idxs' (external_edges (mk_cohg ns es')))
-    (map_to_list ns).*1
-    =ntl= tl2ntl (graph_tensorlist_semantics (mk_cohg ns es')).
-Proof.
-  intros Hes.
-  apply (internal_edges_perm ns) in Hes as Hies.
-  apply (external_edges_perm ns) in Hes as Hees.
-
-  apply perm_exists_perm_seq in Hies as Hidxs.
-  apply perm_exists_perm_seq in Hees as Hidxs'.
-
-  destruct Hidxs as (idxs & Hidxs & Himap).
-  destruct Hidxs' as (idxs' & Hidxs' & Himap').
-  exists idxs, idxs'.
-  split; [easy|].
-  split; [easy|].
-  split.
-  - rewrite <- graph_namedtensorlist_semantics_seq_correct.
-    rewrite graph_namedtensorlist_semantics_to_aux.
-    cbn [nodes].
-    eapply graph_namedtensorlist_semantics_aux_perm_eq';
-    [rewrite fst_zip by (now rewrite length_seq);
-     apply NoDup_seq|..|reflexivity].
-    + etransitivity; [|apply Himap].
-      now rewrite imap_to_zip_with_seq.
-    + etransitivity; [|apply Himap'].
-      now rewrite imap_to_zip_with_seq.
-  - rewrite <- graph_namedtensorlist_semantics_to_aux.
-    rewrite <- graph_namedtensorlist_semantics_seq_correct.
-    apply graph_namedtensorlist_semantics_perm_eq.
-    + rewrite Hidxs; apply NoDup_seq.
-    + rewrite Hidxs.
-      now rewrite length_seq, Hies.
-    + rewrite Hidxs.
-      f_equiv.
-      now rewrite Hies.
-    + rewrite Hidxs'.
-      now rewrite 2 length_seq, Hees.
-Qed.
-
-
-Lemma graph_tensorlist_semantics_perm_eq_pairs ns es es' :
-  es ≡ₚ es' ->
-  exists mid,
-  tl2ntl (graph_tensorlist_semantics (mk_cohg ns es)) ≡ntl'≡ₚ mid /\
-  mid =ntl= tl2ntl (graph_tensorlist_semantics (mk_cohg ns es')).
-Proof.
-  intros Hes.
-  apply (graph_tensorlist_semantics_perm_eq_pairs_elab ns) in Hes.
-  naive_solver.
 Qed.
 
 
